Weidenbach_Book/IsaSAT_Lookup_Conflict.thy
@@ -1623,36 +1623,81 @@ where
 definition (in -) conflict_min_cach :: \<open>nat conflict_min_cach \<Rightarrow> nat \<Rightarrow> minimize_status\<close> where
   [simp]: \<open>conflict_min_cach cach L = cach L\<close>
 
+
+definition lit_redundant_reason_stack2
+  :: \<open>'v literal \<Rightarrow> 'v clauses_l \<Rightarrow> nat \<Rightarrow> (nat \<times> nat \<times> bool)\<close> where
+\<open>lit_redundant_reason_stack2 L NU C' =
+  (if length (NU \<propto> C') > 2 then (C', 1, False)
+  else if NU \<propto> C' ! 0 = L then (C', 1, False)
+  else (C', 0, True))\<close>
+
+definition ana_lookup_rel
+  :: \<open>nat clauses_l \<Rightarrow> ((nat \<times> nat \<times> bool) \<times> (nat \<times> nat \<times> nat \<times> nat)) set\<close>
+where
+\<open>ana_lookup_rel NU = {((C, i, b), (C', k', i', len')).
+  C = C' \<and> k' = (if b then 1 else 0) \<and> i = i' \<and>
+  len' = (if b then 1 else length (NU \<propto> C))}\<close>
+
+lemma ana_lookup_rel_alt_def:
+  \<open>((C, i, b), (C', k', i', len')) \<in> ana_lookup_rel NU \<longleftrightarrow>
+  C = C' \<and> k' = (if b then 1 else 0) \<and> i = i' \<and>
+  len' = (if b then 1 else length (NU \<propto> C))\<close>
+  unfolding ana_lookup_rel_def
+  by auto
+
+abbreviation ana_lookups_rel where
+  \<open>ana_lookups_rel NU \<equiv> \<langle>ana_lookup_rel NU\<rangle>list_rel\<close>
+
+definition ana_lookup_conv :: \<open>nat clauses_l \<Rightarrow> (nat \<times> nat \<times> bool) \<Rightarrow> (nat \<times> nat \<times> nat \<times> nat)\<close> where
+\<open>ana_lookup_conv NU = (\<lambda>(C, i, b). (C, (if b then 1 else 0), i, (if b then 1 else length (NU \<propto> C))))\<close>
+
+definition get_literal_and_remove_of_analyse_wl2
+   :: \<open>'v clause_l \<Rightarrow> (nat \<times> nat \<times> bool) list \<Rightarrow> 'v literal \<times> (nat \<times> nat \<times> bool) list\<close> where
+  \<open>get_literal_and_remove_of_analyse_wl2 C analyse =
+    (let (i, j, b) = last analyse in
+     (C ! j, analyse[length analyse - 1 := (i, j + 1, b)]))\<close>
+
+definition lit_redundant_rec_wl_inv2 where
+  \<open>lit_redundant_rec_wl_inv2 M NU D =
+    (\<lambda>(cach, analyse, b). \<exists>analyse'. (analyse, analyse') \<in> ana_lookups_rel NU \<and>
+      lit_redundant_rec_wl_inv M NU D (cach, analyse', b))\<close>
+
+definition mark_failed_lits_stack_inv2 where
+  \<open>mark_failed_lits_stack_inv2 NU analyse = (\<lambda>cach.
+       \<exists>analyse'. (analyse, analyse') \<in> ana_lookups_rel NU \<and>
+      mark_failed_lits_stack_inv NU analyse' cach)\<close>
+
 definition lit_redundant_rec_wl_lookup
   :: \<open>nat multiset \<Rightarrow> (nat,nat)ann_lits \<Rightarrow> nat clauses_l \<Rightarrow> nat clause \<Rightarrow>
      _ \<Rightarrow> _ \<Rightarrow> _ \<Rightarrow> (_ \<times> _ \<times> bool) nres\<close>
 where
   \<open>lit_redundant_rec_wl_lookup \<A> M NU D cach analysis lbd =
-      WHILE\<^sub>T\<^bsup>lit_redundant_rec_wl_inv M NU D\<^esup>
+      WHILE\<^sub>T\<^bsup>lit_redundant_rec_wl_inv2 M NU D\<^esup>
         (\<lambda>(cach, analyse, b). analyse \<noteq> [])
-        (\<lambda>(cach, (analyse :: (nat \<times> nat \<times> nat \<times> nat) list), b). do {
-            ASSERT((analyse :: (nat \<times> nat \<times> nat \<times> nat) list) \<noteq> []);
-	    let (C,k, i, len) = last analyse;
+        (\<lambda>(cach, analyse, b). do {
+            ASSERT(analyse \<noteq> []);
+	    let (C,k, i, len) = ana_lookup_conv NU (last analyse);
             ASSERT(C \<in># dom_m NU);
             ASSERT(length (NU \<propto> C) > k); \<comment> \<open> >= 2 would work too \<close>
             ASSERT (NU \<propto> C ! k \<in> lits_of_l M);
             ASSERT(NU \<propto> C ! k \<in># \<L>\<^sub>a\<^sub>l\<^sub>l \<A>);
+	    ASSERT(literals_are_in_\<L>\<^sub>i\<^sub>n \<A> (mset (NU \<propto> C)));
 	    ASSERT(len \<le> length (NU \<propto> C)); \<comment> \<open>makes the refinement easier\<close>
             let C = NU \<propto> C;
             if i \<ge> len
             then
                RETURN(cach (atm_of (C ! k) := SEEN_REMOVABLE), butlast analyse, True)
             else do {
-               let (L, analyse) = get_literal_and_remove_of_analyse_wl C analyse;
+               let (L, analyse) = get_literal_and_remove_of_analyse_wl2 C analyse;
                ASSERT(L \<in># \<L>\<^sub>a\<^sub>l\<^sub>l \<A>);
                let b = \<not>level_in_lbd (get_level M L) lbd;
                if (get_level M L = zero_uint32_nat \<or>
                    conflict_min_cach cach (atm_of L) = SEEN_REMOVABLE \<or>
                    atm_in_conflict (atm_of L) D)
-               then RETURN (cach, (analyse :: (nat \<times> nat \<times> nat \<times> nat) list), False)
+               then RETURN (cach, analyse, False)
                else if b \<or> conflict_min_cach cach (atm_of L) = SEEN_FAILED
                then do {
-                  ASSERT(mark_failed_lits_stack_inv NU analyse cach);
+                  ASSERT(mark_failed_lits_stack_inv2 NU analyse cach);
                   cach \<leftarrow> mark_failed_lits_wl NU analyse cach;
                   RETURN (cach, [], False)
                }
@@ -1663,10 +1708,10 @@ where
                     Some C \<Rightarrow> do {
 		      ASSERT(C \<in># dom_m NU);
 		      ASSERT(length (NU \<propto> C) \<ge> 2);
-		      RETURN (cach, analyse @ [lit_redundant_reason_stack (-L) NU C], False)
+		      RETURN (cach, analyse @ [lit_redundant_reason_stack2 (-L) NU C], False)
 		    }
                   | None \<Rightarrow> do {
-                      ASSERT(mark_failed_lits_stack_inv NU analyse cach);
+                      ASSERT(mark_failed_lits_stack_inv2 NU analyse cach);
                       cach \<leftarrow> mark_failed_lits_wl NU analyse cach;
                       RETURN (cach, [], False)
                   }
@@ -1674,6 +1719,11 @@ where
           }
         })
        (cach, analysis, False)\<close>
+
+lemma lit_redundant_rec_wl_ref_butlast:
+  \<open>lit_redundant_rec_wl_ref NU x \<Longrightarrow> lit_redundant_rec_wl_ref NU (butlast x)\<close>
+  by (cases x rule: rev_cases)
+    (auto simp: lit_redundant_rec_wl_ref_def dest: in_set_butlastD)
 
 lemma lit_redundant_rec_wl_lookup_mark_failed_lits_stack_inv:
   assumes
@@ -1696,14 +1746,564 @@ proof -
        (auto simp: elim!: in_set_upd_cases)
 qed
 
+context
+  fixes M D \<A> NU analysis analysis'
+  assumes 
+    M_D: \<open>M \<Turnstile>as CNot D\<close> and
+    n_d: \<open>no_dup M\<close> and
+    lits: \<open>literals_are_in_\<L>\<^sub>i\<^sub>n_trail \<A> M\<close> and
+    ana: \<open>(analysis, analysis') \<in> ana_lookups_rel NU\<close> and
+    lits_NU: \<open>literals_are_in_\<L>\<^sub>i\<^sub>n_mm \<A> ((mset \<circ> fst) `# ran_m NU)\<close>
+begin
+lemma ccmin_rel:
+  assumes \<open>lit_redundant_rec_wl_inv M NU D (cach, analysis', False)\<close>
+  shows \<open>((cach, analysis, False), cach, analysis', False)
+         \<in>  {((cach, ana, b), cach', ana', b').
+          (ana, ana') \<in> ana_lookups_rel NU \<and>
+          b = b' \<and> cach = cach' \<and> lit_redundant_rec_wl_inv M NU D (cach, ana', b)}\<close>
+proof -
+  show ?thesis using ana assms by auto
+qed
+
+
+context
+  fixes x :: \<open>(nat \<Rightarrow> minimize_status) \<times> (nat \<times> nat \<times> bool) list \<times> bool\<close> and
+  x' :: \<open>(nat \<Rightarrow> minimize_status) \<times> (nat \<times> nat \<times> nat \<times> nat) list \<times> bool\<close>
+  assumes x_x': \<open>(x, x') \<in> {((cach, ana, b), (cach', ana', b')).
+     (ana, ana') \<in> ana_lookups_rel NU \<and> b = b' \<and> cach = cach' \<and>
+     lit_redundant_rec_wl_inv M NU D (cach, ana', b)}\<close>
+begin
+
+lemma ccmin_lit_redundant_rec_wl_inv2:
+  assumes \<open>lit_redundant_rec_wl_inv M NU D x'\<close>
+  shows \<open>lit_redundant_rec_wl_inv2 M NU D x\<close>
+  using x_x' unfolding lit_redundant_rec_wl_inv2_def
+  by auto
+
+context
+  assumes 
+    \<open>lit_redundant_rec_wl_inv2 M NU D x\<close> and
+    \<open>lit_redundant_rec_wl_inv M NU D x'\<close>
+begin
+
+lemma ccmin_cond:
+  fixes x1 :: \<open>nat \<Rightarrow> minimize_status\<close> and
+    x2 :: \<open>(nat \<times> nat \<times> bool) list \<times> bool\<close> and
+    x1a :: \<open>(nat \<times>  nat \<times> bool) list\<close> and
+    x2a :: \<open>bool\<close> and x1b :: \<open>nat \<Rightarrow> minimize_status\<close> and
+    x2b :: \<open>(nat \<times> nat \<times> nat \<times> nat) list \<times> bool\<close> and
+    x1c :: \<open>(nat \<times> nat \<times> nat \<times> nat) list\<close> and x2c :: \<open>bool\<close>
+  assumes
+    \<open>x2 = (x1a, x2a)\<close>
+    \<open>x = (x1, x2)\<close>
+    \<open>x2b = (x1c, x2c)\<close>
+    \<open>x' = (x1b, x2b)\<close>
+  shows \<open>(x1a \<noteq> []) = (x1c \<noteq> [])\<close>
+  using assms x_x'
+  by auto
+
+end
+
+
+context
+  assumes 
+    \<open>case x of (cach, analyse, b) \<Rightarrow> analyse \<noteq> []\<close> and
+    \<open>case x' of (cach, analyse, b) \<Rightarrow> analyse \<noteq> []\<close> and
+    inv2: \<open>lit_redundant_rec_wl_inv2 M NU D x\<close> and
+    \<open>lit_redundant_rec_wl_inv M NU D x'\<close>
+begin
+
+context
+  fixes x1 :: \<open>nat \<Rightarrow> minimize_status\<close> and
+  x2 :: \<open>(nat \<times> nat \<times> nat \<times> nat) list \<times> bool\<close> and
+  x1a :: \<open>(nat \<times> nat \<times> nat \<times> nat) list\<close> and x2a :: \<open>bool\<close> and
+  x1b :: \<open>nat \<Rightarrow> minimize_status\<close> and
+  x2b :: \<open>(nat \<times> nat \<times> bool) list \<times> bool\<close> and
+  x1c :: \<open>(nat \<times> nat \<times> bool) list\<close> and
+  x2c :: \<open>bool\<close>
+  assumes st:
+    \<open>x2 = (x1a, x2a)\<close>
+    \<open>x' = (x1, x2)\<close>
+    \<open>x2b = (x1c, x2c)\<close>
+    \<open>x = (x1b, x2b)\<close> and
+    x1a: \<open>x1a \<noteq> []\<close>
+begin
+
+private lemma st:
+    \<open>x2 = (x1a, x2a)\<close>
+    \<open>x' = (x1, x1a, x2a)\<close>
+    \<open>x2b = (x1c, x2a)\<close>
+    \<open>x = (x1, x1c, x2a)\<close>
+    \<open>x1b = x1\<close>
+    \<open>x2c = x2a\<close> and
+  x1c: \<open>x1c \<noteq> []\<close>
+  using st x_x' x1a by auto
+
+lemma ccmin_nempty:
+  shows \<open>x1c \<noteq> []\<close>
+  using x_x' x1a
+  by (auto simp: st)
+
+context
+  notes _[simp] = st
+  fixes x1d :: \<open>nat\<close> and x2d :: \<open>nat \<times> nat \<times> nat\<close> and
+    x1e :: \<open>nat\<close> and x2e :: \<open>nat \<times> nat\<close> and
+    x1f :: \<open>nat\<close> and
+    x2f :: \<open>nat\<close> and x1g :: \<open>nat\<close> and
+    x2g :: \<open>nat \<times> nat \<times> nat\<close> and
+    x1h :: \<open>nat\<close> and
+    x2h :: \<open>nat \<times> nat\<close> and
+    x1i :: \<open>nat\<close> and
+    x2i :: \<open>nat\<close>
+  assumes
+    ana_lookup_conv: \<open>ana_lookup_conv NU (last x1c) = (x1g, x2g)\<close> and
+    last: \<open>last x1a = (x1d, x2d)\<close> and
+    dom: \<open>x1d \<in># dom_m NU\<close> and
+    le: \<open>x1e < length (NU \<propto> x1d)\<close> and
+    in_lits: \<open>NU \<propto> x1d ! x1e \<in> lits_of_l M\<close> and
+    st2:
+      \<open>x2g = (x1h, x2h)\<close>
+      \<open>x2e = (x1f, x2f)\<close>
+      \<open>x2d = (x1e, x2e)\<close>
+      \<open>x2h = (x1i, x2i)\<close>
+begin
+
+private lemma x1g_x1d:
+    \<open>x1g = x1d\<close>
+    \<open>x1h = x1e\<close>
+    \<open>x1i = x1f\<close>
+  using st2 last ana_lookup_conv x_x' x1a last
+  by (cases x1a rule: rev_cases; cases x1c rule: rev_cases;
+    auto simp: ana_lookup_conv_def ana_lookup_rel_def
+      list_rel_append_single_iff; fail)+
+
+private definition j where
+  \<open>j = fst (snd (last x1c))\<close>
+
+private definition b where
+  \<open>b = snd (snd (last x1c))\<close>
+
+private lemma last_x1c[simp]:
+  \<open>last x1c = (x1d, x1f, b)\<close>
+  using inv2 x1a last x_x' unfolding x1g_x1d st j_def b_def st2
+  by (cases x1a rule: rev_cases; cases x1c rule: rev_cases;
+   auto simp: lit_redundant_rec_wl_inv2_def list_rel_append_single_iff
+    lit_redundant_rec_wl_inv_def ana_lookup_rel_def
+    lit_redundant_rec_wl_ref_def)
+
+private lemma
+  ana: \<open>(x1d, (if b then 1 else 0), x1f, (if b then 1 else length (NU \<propto> x1d))) = (x1d, x1e, x1f, x2i)\<close> and
+  st3:
+    \<open>x1e = (if b then 1 else 0)\<close>
+    \<open>x1f = j\<close>
+    \<open>x2f = (if b then 1 else length (NU \<propto> x1d))\<close>
+    \<open>x2d = (if b then 1 else 0, j, if b then 1 else length (NU \<propto> x1d))\<close> and
+    \<open>j \<le> (if b then 1 else length (NU \<propto> x1d))\<close> and
+    \<open>x1d \<in># dom_m NU\<close> and
+    \<open>0 < x1d\<close> and
+    \<open>(if b then 1 else length (NU \<propto> x1d)) \<le> length (NU \<propto> x1d)\<close> and
+    \<open>(if b then 1 else 0) < length (NU \<propto> x1d)\<close> and
+    dist: \<open>distinct (NU \<propto> x1d)\<close> and
+    tauto: \<open>\<not> tautology (mset (NU \<propto> x1d))\<close>
+  subgoal
+    using inv2 x1a last x_x' x1c ana_lookup_conv
+    unfolding x1g_x1d st j_def b_def st2
+    by (cases x1a rule: rev_cases; cases x1c rule: rev_cases;
+     auto simp: lit_redundant_rec_wl_inv2_def list_rel_append_single_iff
+         lit_redundant_rec_wl_inv_def ana_lookup_rel_def
+         lit_redundant_rec_wl_ref_def ana_lookup_conv_def
+       simp del: x1c)
+  subgoal
+    using inv2 x1a last x_x' x1c unfolding x1g_x1d st j_def b_def st2
+    by (cases x1a rule: rev_cases; cases x1c rule: rev_cases;
+     auto simp: lit_redundant_rec_wl_inv2_def list_rel_append_single_iff
+         lit_redundant_rec_wl_inv_def ana_lookup_rel_def
+         lit_redundant_rec_wl_ref_def
+       simp del: x1c)
+  subgoal
+    using inv2 x1a last x_x' x1c unfolding x1g_x1d st j_def b_def st2
+    by (cases x1a rule: rev_cases; cases x1c rule: rev_cases;
+     auto simp: lit_redundant_rec_wl_inv2_def list_rel_append_single_iff
+         lit_redundant_rec_wl_inv_def ana_lookup_rel_def
+         lit_redundant_rec_wl_ref_def
+       simp del: x1c)
+  subgoal
+    using inv2 x1a last x_x' x1c unfolding x1g_x1d st j_def b_def st2
+    by (cases x1a rule: rev_cases; cases x1c rule: rev_cases;
+     auto simp: lit_redundant_rec_wl_inv2_def list_rel_append_single_iff
+         lit_redundant_rec_wl_inv_def ana_lookup_rel_def
+         lit_redundant_rec_wl_ref_def
+       simp del: x1c)
+  subgoal
+    using inv2 x1a last x_x' x1c unfolding x1g_x1d st j_def b_def st2
+    by (cases x1a rule: rev_cases; cases x1c rule: rev_cases;
+     auto simp: lit_redundant_rec_wl_inv2_def list_rel_append_single_iff
+         lit_redundant_rec_wl_inv_def ana_lookup_rel_def
+         lit_redundant_rec_wl_ref_def
+       simp del: x1c)
+  subgoal
+    using inv2 x1a last x_x' x1c unfolding x1g_x1d st j_def b_def st2
+    by (cases x1a rule: rev_cases; cases x1c rule: rev_cases;
+     auto simp: lit_redundant_rec_wl_inv2_def list_rel_append_single_iff
+         lit_redundant_rec_wl_inv_def ana_lookup_rel_def
+         lit_redundant_rec_wl_ref_def
+       simp del: x1c)
+  subgoal
+    using inv2 x1a last x_x' x1c unfolding x1g_x1d st j_def b_def
+    by (cases x1a rule: rev_cases; cases x1c rule: rev_cases;
+     auto simp: lit_redundant_rec_wl_inv2_def list_rel_append_single_iff
+         lit_redundant_rec_wl_inv_def ana_lookup_rel_def
+         lit_redundant_rec_wl_ref_def
+       simp del: x1c)
+  subgoal
+    using inv2 x1a last x_x' x1c unfolding x1g_x1d st j_def b_def
+    by (cases x1a rule: rev_cases; cases x1c rule: rev_cases;
+     auto simp: lit_redundant_rec_wl_inv2_def list_rel_append_single_iff
+         lit_redundant_rec_wl_inv_def ana_lookup_rel_def
+         lit_redundant_rec_wl_ref_def
+       simp del: x1c)
+  subgoal
+    using inv2 x1a last x_x' x1c unfolding x1g_x1d st j_def b_def
+    by (cases x1a rule: rev_cases; cases x1c rule: rev_cases;
+     auto simp: lit_redundant_rec_wl_inv2_def list_rel_append_single_iff
+         lit_redundant_rec_wl_inv_def ana_lookup_rel_def
+         lit_redundant_rec_wl_ref_def
+       simp del: x1c)
+  subgoal
+    using inv2 x1a last x_x' x1c unfolding x1g_x1d st j_def b_def
+    by (cases x1a rule: rev_cases; cases x1c rule: rev_cases;
+     auto simp: lit_redundant_rec_wl_inv2_def list_rel_append_single_iff
+         lit_redundant_rec_wl_inv_def ana_lookup_rel_def
+         lit_redundant_rec_wl_ref_def
+       simp del: x1c)
+  subgoal
+    using inv2 x1a last x_x' x1c unfolding x1g_x1d st j_def b_def
+    by (cases x1a rule: rev_cases; cases x1c rule: rev_cases;
+     auto simp: lit_redundant_rec_wl_inv2_def list_rel_append_single_iff
+         lit_redundant_rec_wl_inv_def ana_lookup_rel_def
+         lit_redundant_rec_wl_ref_def
+       simp del: x1c)
+  subgoal
+    using inv2 x1a last x_x' x1c unfolding x1g_x1d st j_def b_def
+    by (cases x1a rule: rev_cases; cases x1c rule: rev_cases;
+     auto simp: lit_redundant_rec_wl_inv2_def list_rel_append_single_iff
+         lit_redundant_rec_wl_inv_def ana_lookup_rel_def
+         lit_redundant_rec_wl_ref_def
+       simp del: x1c)
+  done
+
+lemma ccmin_in_dom:
+  shows x1g_dom: \<open>x1g \<in># dom_m NU\<close>
+  using dom unfolding x1g_x1d .
+
+lemma ccmin_in_dom_le_length:
+  shows \<open>x1h < length (NU \<propto> x1g)\<close>
+  using le unfolding x1g_x1d .
+
+lemma ccmin_in_trail:
+  shows \<open>NU \<propto> x1g ! x1h \<in> lits_of_l M\<close>
+  using in_lits unfolding x1g_x1d .
+
+lemma ccmin_literals_are_in_\<L>\<^sub>i\<^sub>n_NU_x1g:
+  shows \<open>literals_are_in_\<L>\<^sub>i\<^sub>n \<A> (mset (NU \<propto> x1g))\<close>
+  using lits_NU multi_member_split[OF x1g_dom]
+  by (auto simp: ran_m_def literals_are_in_\<L>\<^sub>i\<^sub>n_mm_add_mset)
+
+lemma ccmin_in_all_lits:
+  shows \<open>NU \<propto> x1g ! x1h \<in># \<L>\<^sub>a\<^sub>l\<^sub>l \<A>\<close>
+  using literals_are_in_\<L>\<^sub>i\<^sub>n_in_\<L>\<^sub>a\<^sub>l\<^sub>l[OF ccmin_literals_are_in_\<L>\<^sub>i\<^sub>n_NU_x1g, of x1h]
+  le unfolding x1g_x1d by auto
+
+lemma ccmin_less_length:
+  shows \<open>x2i \<le> length (NU \<propto> x1g)\<close>
+  using le ana unfolding x1g_x1d st3 by (simp split: if_splits)
+
+lemma ccmin_same_cond:
+  shows \<open>(x2i \<le> x1i) = (x2f \<le> x1f)\<close>
+  using le ana unfolding x1g_x1d st3 by (simp split: if_splits)
+
+lemma ccmin_set_removable:
+  assumes 
+    \<open>x2i \<le> x1i\<close> and
+    \<open>x2f \<le> x1f\<close>
+  shows \<open>((x1b(atm_of (NU \<propto> x1g ! x1h) := SEEN_REMOVABLE), butlast x1c, True),
+          x1(atm_of (NU \<propto> x1d ! x1e) := SEEN_REMOVABLE), butlast x1a, True)
+         \<in> {((cach, ana, b), cach', ana', b').
+       (ana, ana') \<in> ana_lookups_rel NU \<and>
+       b = b' \<and> cach = cach' \<and> lit_redundant_rec_wl_inv M NU D (cach, ana', b)}\<close>
+  using x_x' by (auto simp: x1g_x1d lit_redundant_rec_wl_ref_butlast lit_redundant_rec_wl_inv_def
+    dest: list_rel_butlast)
+
+context
+  assumes 
+    le: \<open>\<not> x2i \<le> x1i\<close> \<open>\<not> x2f \<le> x1f\<close>
+begin
+
+context
+  notes _[simp]= x1g_x1d st2 last
+  fixes x1j :: \<open>nat literal\<close> and x2j :: \<open>(nat \<times> nat \<times> nat \<times> nat) list\<close> and
+  x1k :: \<open>nat literal\<close> and x2k :: \<open>(nat \<times> nat \<times> bool) list\<close>
+  assumes 
+    rem: \<open>get_literal_and_remove_of_analyse_wl (NU \<propto> x1d) x1a = (x1j, x2j)\<close> and
+    rem2:\<open>get_literal_and_remove_of_analyse_wl2 (NU \<propto> x1g) x1c = (x1k, x2k)\<close> and
+    \<open>fst (snd (snd (last x2j))) \<noteq> 0\<close> and
+    ux1j_M: \<open>- x1j \<in> lits_of_l M\<close>
+begin
+
+private lemma confl_min_last: \<open>(last x1c, last x1a) \<in> ana_lookup_rel NU\<close>
+  using x1a x1c x_x' rem rem2 last ana_lookup_conv unfolding x1g_x1d st2 b_def st
+  by (cases x1c rule: rev_cases; cases x1a rule: rev_cases)
+    (auto simp: list_rel_append_single_iff
+     get_literal_and_remove_of_analyse_wl_def
+    get_literal_and_remove_of_analyse_wl2_def)
+
+private lemma rel: \<open>(x1c[length x1c - Suc 0 := (x1d, Suc x1f, b)], x1a
+     [length x1a - Suc 0 := (x1d, x1e, Suc x1f, x2f)])
+    \<in> ana_lookups_rel NU\<close>
+  using x1a x1c x_x' rem rem2 confl_min_last unfolding x1g_x1d st2 last b_def st
+  by (cases x1c rule: rev_cases; cases x1a rule: rev_cases)
+    (auto simp: list_rel_append_single_iff
+      ana_lookup_rel_alt_def get_literal_and_remove_of_analyse_wl_def
+      get_literal_and_remove_of_analyse_wl2_def)
+
+private lemma x1k_x1j: \<open>x1k = x1j\<close> \<open>x1j = NU \<propto> x1d ! x1f\<close> and
+  x2k_x2j: \<open>(x2k, x2j) \<in> ana_lookups_rel NU\<close>
+  subgoal
+    using x1a x1c x_x' rem rem2 confl_min_last unfolding x1g_x1d st2 last b_def st
+    by (cases x1c rule: rev_cases; cases x1a rule: rev_cases)
+      (auto simp: list_rel_append_single_iff
+	ana_lookup_rel_alt_def get_literal_and_remove_of_analyse_wl_def
+	get_literal_and_remove_of_analyse_wl2_def)
+  subgoal
+    using x1a x1c x_x' rem rem2 confl_min_last unfolding x1g_x1d st2 last b_def st
+    by (cases x1c rule: rev_cases; cases x1a rule: rev_cases)
+      (auto simp: list_rel_append_single_iff
+	ana_lookup_rel_alt_def get_literal_and_remove_of_analyse_wl_def
+	get_literal_and_remove_of_analyse_wl2_def)
+  subgoal
+    using x1a x1c x_x' rem rem2 confl_min_last unfolding x1g_x1d st2 last b_def st
+    by (cases x1c rule: rev_cases; cases x1a rule: rev_cases)
+      (auto simp: list_rel_append_single_iff
+	ana_lookup_rel_alt_def get_literal_and_remove_of_analyse_wl_def
+	get_literal_and_remove_of_analyse_wl2_def)
+  done
+
+lemma ccmin_x1k_all:
+  shows \<open>x1k \<in># \<L>\<^sub>a\<^sub>l\<^sub>l \<A>\<close>
+  unfolding x1k_x1j
+  using literals_are_in_\<L>\<^sub>i\<^sub>n_in_\<L>\<^sub>a\<^sub>l\<^sub>l[OF ccmin_literals_are_in_\<L>\<^sub>i\<^sub>n_NU_x1g, of x1f]
+    literals_are_in_\<L>\<^sub>i\<^sub>n_trail_in_lits_of_l[OF lits \<open>- x1j \<in> lits_of_l M\<close>]
+  le st3 unfolding x1g_x1d by (auto split: if_splits simp: x1k_x1j uminus_\<A>\<^sub>i\<^sub>n_iff)
+
+
+context
+  notes _[simp]= x1k_x1j
+  fixes b :: \<open>bool\<close> and lbd
+  assumes b: \<open>(\<not> level_in_lbd (get_level M x1k) lbd, b) \<in> bool_rel\<close>
+begin
+
+private lemma in_conflict_atm_in:
+  \<open>- x1e' \<in> lits_of_l M \<Longrightarrow> atm_in_conflict (atm_of x1e') D \<longleftrightarrow> x1e' \<in># D\<close> for x1e'
+  using M_D n_d
+  by (auto simp: atm_in_conflict_def true_annots_true_cls_def_iff_negation_in_model
+      atms_of_def atm_of_eq_atm_of dest!: multi_member_split no_dup_consistentD)
+
+lemma ccmin_already_seen:
+  shows \<open>(get_level M x1k = zero_uint32_nat \<or>
+          conflict_min_cach x1b (atm_of x1k) = SEEN_REMOVABLE \<or>
+          atm_in_conflict (atm_of x1k) D) =
+         (get_level M x1j = 0 \<or> x1 (atm_of x1j) = SEEN_REMOVABLE \<or> x1j \<in># D)\<close>
+  using in_lits ana ux1j_M
+  by (auto simp add: in_conflict_atm_in)
+
+
+private lemma ccmin_lit_redundant_rec_wl_inv: \<open>lit_redundant_rec_wl_inv M NU D
+     (x1, x2j, False)\<close>
+  using x_x' last ana_lookup_conv rem rem2 x1a x1c le
+  by (cases x1a rule: rev_cases; cases x1c rule: rev_cases)
+    (auto simp add: lit_redundant_rec_wl_inv_def lit_redundant_rec_wl_ref_def
+    lit_redundant_reason_stack_def get_literal_and_remove_of_analyse_wl_def
+    list_rel_append_single_iff get_literal_and_remove_of_analyse_wl2_def)
+ 
+lemma ccmin_already_seen_rel:
+  assumes 
+    \<open>get_level M x1k = zero_uint32_nat \<or>
+     conflict_min_cach x1b (atm_of x1k) = SEEN_REMOVABLE \<or>
+     atm_in_conflict (atm_of x1k) D\<close> and
+    \<open>get_level M x1j = 0 \<or> x1 (atm_of x1j) = SEEN_REMOVABLE \<or> x1j \<in># D\<close>
+  shows \<open>((x1b, x2k, False), x1, x2j, False)
+         \<in> {((cach, ana, b), cach', ana', b').
+          (ana, ana') \<in> ana_lookups_rel NU \<and>
+          b = b' \<and> cach = cach' \<and> lit_redundant_rec_wl_inv M NU D (cach, ana', b)}\<close>
+  using x2k_x2j ccmin_lit_redundant_rec_wl_inv by auto
+
+context
+  assumes 
+    \<open>\<not> (get_level M x1k = zero_uint32_nat \<or>
+        conflict_min_cach x1b (atm_of x1k) = SEEN_REMOVABLE \<or>
+        atm_in_conflict (atm_of x1k) D)\<close> and
+    \<open>\<not> (get_level M x1j = 0 \<or> x1 (atm_of x1j) = SEEN_REMOVABLE \<or> x1j \<in># D)\<close>
+begin
+lemma ccmin_already_failed:
+  shows \<open>(\<not> level_in_lbd (get_level M x1k) lbd \<or>
+          conflict_min_cach x1b (atm_of x1k) = SEEN_FAILED) =
+         (b \<or> x1 (atm_of x1j) = SEEN_FAILED)\<close>
+  using b by auto
+
+
+context
+  assumes 
+    \<open>\<not> level_in_lbd (get_level M x1k) lbd \<or>
+     conflict_min_cach x1b (atm_of x1k) = SEEN_FAILED\<close> and
+    \<open>b \<or> x1 (atm_of x1j) = SEEN_FAILED\<close>
+begin
+
+lemma ccmin_mark_failed_lits_stack_inv2_lbd:
+  shows \<open>mark_failed_lits_stack_inv2 NU x2k x1b\<close>
+  using x1a x1c x2k_x2j rem rem2 x_x' le last
+  unfolding mark_failed_lits_stack_inv_def lit_redundant_rec_wl_inv_def
+    lit_redundant_rec_wl_ref_def get_literal_and_remove_of_analyse_wl_def
+  unfolding mark_failed_lits_stack_inv2_def
+  apply -
+  apply (rule exI[of _ x2j])
+  apply (cases \<open>x1a\<close> rule: rev_cases; cases \<open>x1c\<close> rule: rev_cases)
+  by (auto simp: mark_failed_lits_stack_inv_def elim!: in_set_upd_cases)
+
+lemma ccmin_mark_failed_lits_wl_lbd:
+  shows \<open>mark_failed_lits_wl NU x2k x1b
+         \<le> \<Down> Id
+            (mark_failed_lits_wl NU x2j x1)\<close>	  
+  by (auto simp: mark_failed_lits_wl_def)
+
+
+lemma ccmin_rel_lbd:
+  fixes cach :: \<open>nat \<Rightarrow> minimize_status\<close> and cacha :: \<open>nat \<Rightarrow> minimize_status\<close>
+  assumes \<open>(cach, cacha)  \<in> Id\<close>
+  shows \<open>((cach, [], False), cacha, [], False) \<in> {((cach, ana, b), cach', ana', b').
+       (ana, ana') \<in> ana_lookups_rel NU \<and>
+       b = b' \<and> cach = cach' \<and> lit_redundant_rec_wl_inv M NU D (cach, ana', b)}\<close>
+  using x_x' assms by (auto simp: lit_redundant_rec_wl_inv_def lit_redundant_rec_wl_ref_def)
+
+end
+
+
+context
+  assumes 
+    \<open>\<not> (\<not> level_in_lbd (get_level M x1k) lbd \<or>
+        conflict_min_cach x1b (atm_of x1k) = SEEN_FAILED)\<close> and
+    \<open>\<not> (b \<or> x1 (atm_of x1j) = SEEN_FAILED)\<close>
+begin
+
+lemma ccmin_lit_in_trail:
+  \<open>- x1k \<in> lits_of_l M\<close>
+  using \<open>- x1j \<in> lits_of_l M\<close> x1k_x1j(1) by blast 
+
+lemma ccmin_lit_eq:
+  \<open>- x1k = - x1j\<close>
+  by auto
+
+
+context
+  fixes xa :: \<open>nat option\<close> and x'a :: \<open>nat option\<close>
+  assumes xa_x'a: \<open>(xa, x'a) \<in> \<langle>nat_rel\<rangle>option_rel\<close>
+begin
+
+lemma ccmin_lit_eq2:
+  \<open>(xa, x'a) \<in> Id\<close>
+  using xa_x'a by auto
+
+context
+  assumes 
+    [simp]: \<open>xa = None\<close> \<open>x'a = None\<close>
+begin
+
+lemma ccmin_mark_failed_lits_stack_inv2_dec:
+  \<open>mark_failed_lits_stack_inv2 NU x2k x1b\<close>
+  using x1a x1c x2k_x2j rem rem2 x_x' le last
+  unfolding mark_failed_lits_stack_inv_def lit_redundant_rec_wl_inv_def
+    lit_redundant_rec_wl_ref_def get_literal_and_remove_of_analyse_wl_def
+  unfolding mark_failed_lits_stack_inv2_def
+  apply -
+  apply (rule exI[of _ x2j])
+  apply (cases \<open>x1a\<close> rule: rev_cases; cases \<open>x1c\<close> rule: rev_cases)
+  by (auto simp: mark_failed_lits_stack_inv_def elim!: in_set_upd_cases)
+
+lemma ccmin_mark_failed_lits_stack_wl_dec:
+  shows \<open>mark_failed_lits_wl NU x2k x1b
+         \<le> \<Down> Id
+            (mark_failed_lits_wl NU x2j x1)\<close>
+  by (auto simp: mark_failed_lits_wl_def)
+
+
+lemma ccmin_rel_dec:
+  fixes cach :: \<open>nat \<Rightarrow> minimize_status\<close> and cacha :: \<open>nat \<Rightarrow> minimize_status\<close>
+  assumes \<open>(cach, cacha)  \<in> Id\<close>
+  shows \<open>((cach, [], False), cacha, [], False)
+         \<in>  {((cach, ana, b), cach', ana', b').
+       (ana, ana') \<in> ana_lookups_rel NU \<and>
+       b = b' \<and> cach = cach' \<and> lit_redundant_rec_wl_inv M NU D (cach, ana', b)}\<close>
+  using assms by (auto simp: lit_redundant_rec_wl_ref_def lit_redundant_rec_wl_inv_def)
+
+end
+
+
+context
+  fixes xb :: \<open>nat\<close> and x'b :: \<open>nat\<close>
+  assumes H:
+    \<open>xa = Some xb\<close>
+    \<open>x'a = Some x'b\<close>
+    \<open>(xb, x'b) \<in> nat_rel\<close>
+    \<open>x'b \<in># dom_m NU\<close>
+    \<open>2 \<le> length (NU \<propto> x'b)\<close>
+    \<open>x'b > 0\<close>
+    \<open>distinct (NU \<propto> x'b) \<and> \<not> tautology (mset (NU \<propto> x'b))\<close>
+begin
+
+lemma ccmin_stack_pre:
+  shows \<open>xb \<in># dom_m NU\<close> \<open>2 \<le> length (NU \<propto> xb)\<close>
+  using H by auto
+
+private lemma ccmin_lit_redundant_rec_wl_inv3: \<open>lit_redundant_rec_wl_inv M NU D
+     (x1, x2j @ [lit_redundant_reason_stack (- NU \<propto> x1d ! x1f) NU x'b], False)\<close>
+  using ccmin_stack_pre H x_x' last ana_lookup_conv rem rem2 x1a x1c le
+  by (cases x1a rule: rev_cases; cases x1c rule: rev_cases)
+    (auto simp add: lit_redundant_rec_wl_inv_def lit_redundant_rec_wl_ref_def
+    lit_redundant_reason_stack_def get_literal_and_remove_of_analyse_wl_def
+    list_rel_append_single_iff get_literal_and_remove_of_analyse_wl2_def)
+
+lemma ccmin_stack_rel:
+  shows \<open>((x1b, x2k @ [lit_redundant_reason_stack2 (- x1k) NU xb], False), x1,
+          x2j @ [lit_redundant_reason_stack (- x1j) NU x'b], False)
+         \<in>  {((cach, ana, b), cach', ana', b').
+       (ana, ana') \<in> ana_lookups_rel NU \<and>
+       b = b' \<and> cach = cach' \<and> lit_redundant_rec_wl_inv M NU D (cach, ana', b)}\<close>
+  using x2k_x2j H ccmin_lit_redundant_rec_wl_inv3
+  by (auto simp: list_rel_append_single_iff ana_lookup_rel_alt_def
+      lit_redundant_reason_stack2_def lit_redundant_reason_stack_def)
+
+end
+end
+end
+end
+end
+end
+end
+end
+end
+end
+end
+end
+
 lemma lit_redundant_rec_wl_lookup_lit_redundant_rec_wl:
   assumes
     M_D: \<open>M \<Turnstile>as CNot D\<close> and
     n_d: \<open>no_dup M\<close> and
-    lits: \<open>literals_are_in_\<L>\<^sub>i\<^sub>n_trail \<A> M\<close>
+    lits: \<open>literals_are_in_\<L>\<^sub>i\<^sub>n_trail \<A> M\<close> and
+    \<open>(analysis, analysis') \<in> ana_lookups_rel NU\<close> and
+    \<open>literals_are_in_\<L>\<^sub>i\<^sub>n_mm \<A> ((mset \<circ> fst) `# ran_m NU)\<close>
   shows
    \<open>lit_redundant_rec_wl_lookup \<A> M NU D cach analysis lbd \<le>
-      \<Down> Id (lit_redundant_rec_wl M NU D cach analysis lbd)\<close>
+      \<Down> (Id \<times>\<^sub>r (ana_lookups_rel NU) \<times>\<^sub>r bool_rel) (lit_redundant_rec_wl M NU D cach analysis' lbd)\<close>
 proof -
   have M: \<open>\<forall>a \<in> lits_of_l M. a \<in># \<L>\<^sub>a\<^sub>l\<^sub>l \<A>\<close>
     using literals_are_in_\<L>\<^sub>i\<^sub>n_trail_in_lits_of_l lits by blast
@@ -1727,46 +2327,46 @@ proof -
         (mark_failed_lits_wl NU a' b')\<close> if \<open>a = a'\<close> and \<open>b = b'\<close> for a a' b b'
     unfolding that by auto
 
-  show ?thesis
+  have H: \<open>lit_redundant_rec_wl_lookup \<A> M NU D cach analysis lbd \<le>
+      \<Down> {((cach, ana, b), cach', ana', b').
+          (ana, ana') \<in> ana_lookups_rel NU \<and>
+          b = b' \<and> cach = cach' \<and> lit_redundant_rec_wl_inv M NU D (cach, ana', b)}
+       (lit_redundant_rec_wl M NU D cach analysis' lbd)\<close>
+    using assms apply -
     unfolding lit_redundant_rec_wl_lookup_def lit_redundant_rec_wl_def WHILET_def
     apply (refine_vcg)
-    subgoal by auto
-    subgoal by (auto simp: lit_redundant_rec_wl_inv_def
-          lit_redundant_rec_wl_ref_def)
-    subgoal by auto
-    subgoal by auto
-    subgoal by (auto simp: lit_redundant_rec_wl_inv_def lit_redundant_rec_wl_ref_def
-          elim!: neq_Nil_revE)
-    subgoal by (auto simp: lit_redundant_rec_wl_inv_def elim!: neq_Nil_revE)
-    subgoal by auto
-    subgoal for x x' x1 x2 x1a x2a x1b x2b x1c x2c
-      unfolding lit_redundant_rec_wl_inv_def lit_redundant_rec_wl_ref_def
-      by (auto simp: lit_redundant_rec_wl_inv_def elim!: neq_Nil_revE[of x1a])
-    subgoal by (auto simp: lit_redundant_rec_wl_inv_def lit_redundant_rec_wl_ref_def
-          elim!: neq_Nil_revE)
-    subgoal by (auto simp: lit_redundant_rec_wl_inv_def lit_redundant_rec_wl_ref_def
-          elim!: neq_Nil_revE)
-    subgoal by auto
-    subgoal by auto
-    subgoal by (auto intro!:)
-    subgoal by auto
-    subgoal by auto
-    subgoal by (rule lit_redundant_rec_wl_lookup_mark_failed_lits_stack_inv; assumption?)
-        (auto)
-    subgoal by auto
-    subgoal by auto
-    subgoal by auto
-    subgoal by auto
-    subgoal by auto
-    subgoal by auto
-    subgoal by (rule lit_redundant_rec_wl_lookup_mark_failed_lits_stack_inv) auto
-    subgoal by auto
-    subgoal by auto
-    subgoal by auto
-    subgoal by auto
-    subgoal by auto
-    subgoal by auto
+    subgoal by (rule ccmin_rel)
+    subgoal by (rule ccmin_lit_redundant_rec_wl_inv2)
+    subgoal by (rule ccmin_cond)
+    subgoal by (rule ccmin_nempty)
+    subgoal by (rule ccmin_in_dom)
+    subgoal by (rule ccmin_in_dom_le_length)
+    subgoal by (rule ccmin_in_trail)
+    subgoal by (rule ccmin_in_all_lits)
+    subgoal by (rule ccmin_literals_are_in_\<L>\<^sub>i\<^sub>n_NU_x1g)
+    subgoal by (rule ccmin_less_length)
+    subgoal by (rule ccmin_same_cond)
+    subgoal by (rule ccmin_set_removable)
+    subgoal by (rule ccmin_x1k_all)
+    subgoal by (rule ccmin_already_seen)
+    subgoal by (rule ccmin_already_seen_rel)
+    subgoal by (rule ccmin_already_failed)
+    subgoal by (rule ccmin_mark_failed_lits_stack_inv2_lbd)
+    apply (rule ccmin_mark_failed_lits_wl_lbd; assumption)
+    subgoal by (rule ccmin_rel_lbd)
+    subgoal by (rule ccmin_lit_in_trail)
+    subgoal by (rule ccmin_lit_eq)
+    subgoal by (rule ccmin_lit_eq2)
+    subgoal by (rule ccmin_mark_failed_lits_stack_inv2_dec)
+    apply (rule ccmin_mark_failed_lits_stack_wl_dec; assumption)
+    subgoal by (rule ccmin_rel_dec)
+    subgoal by (rule ccmin_stack_pre)
+    subgoal by (rule ccmin_stack_pre)
+    subgoal by (rule ccmin_stack_rel)
     done
+  show ?thesis
+    by (rule H[THEN order_trans], rule conc_fun_R_mono)
+     auto
 qed
 
 
@@ -1784,7 +2384,8 @@ definition literal_redundant_wl_lookup where
          Some C \<Rightarrow> do {
 	   ASSERT(C \<in># dom_m NU);
 	   ASSERT(length (NU \<propto> C) \<ge> 2);
-	   lit_redundant_rec_wl_lookup \<A> M NU D cach [lit_redundant_reason_stack (-L) NU C] lbd
+	   ASSERT(distinct (NU \<propto> C) \<and> \<not>tautology (mset (NU \<propto> C)));
+	   lit_redundant_rec_wl_lookup \<A> M NU D cach [lit_redundant_reason_stack2 (-L) NU C] lbd
 	 }
        | None \<Rightarrow> do {
            RETURN (cach, [], False)
@@ -1794,8 +2395,10 @@ definition literal_redundant_wl_lookup where
 
 lemma literal_redundant_wl_lookup_literal_redundant_wl:
   assumes \<open>M \<Turnstile>as CNot D\<close> \<open>no_dup M\<close> \<open>literals_are_in_\<L>\<^sub>i\<^sub>n_trail \<A> M\<close>
+    \<open>literals_are_in_\<L>\<^sub>i\<^sub>n_mm \<A> ((mset \<circ> fst) `# ran_m NU)\<close>
   shows
-    \<open>literal_redundant_wl_lookup \<A> M NU D cach L lbd \<le> \<Down> Id (literal_redundant_wl M NU D cach L lbd)\<close>
+    \<open>literal_redundant_wl_lookup \<A> M NU D cach L lbd \<le>
+      \<Down> (Id \<times>\<^sub>f (ana_lookups_rel NU \<times>\<^sub>f bool_rel)) (literal_redundant_wl M NU D cach L lbd)\<close>
 proof -
   have M: \<open>\<forall>a \<in> lits_of_l M. a \<in># \<L>\<^sub>a\<^sub>l\<^sub>l \<A>\<close>
     using literals_are_in_\<L>\<^sub>i\<^sub>n_trail_in_lits_of_l assms by blast
@@ -1817,13 +2420,17 @@ proof -
     subgoal by auto
     subgoal by auto
     subgoal by auto
-    subgoal for x x' xa x'a
-      apply (subgoal_tac \<open>lit_redundant_rec_wl_lookup \<A> M NU D cach [lit_redundant_reason_stack (-L) NU xa] lbd
-    \<le> \<Down> Id (lit_redundant_rec_wl M NU D cach [lit_redundant_reason_stack (-L) NU xa] lbd)\<close>)
-      subgoal by simp
-      subgoal using assms
-        by (rule lit_redundant_rec_wl_lookup_lit_redundant_rec_wl)
-      done
+    subgoal by auto
+    subgoal by auto
+    subgoal by auto
+    subgoal by auto
+    subgoal by auto
+    subgoal using assms by auto
+    subgoal using assms by auto
+    subgoal using assms by auto
+    subgoal by (auto simp: lit_redundant_reason_stack2_def lit_redundant_reason_stack_def
+      ana_lookup_rel_def)
+    subgoal using assms by auto
     done
 qed
 
@@ -1905,6 +2512,7 @@ lemma minimize_and_extract_highest_lookup_conflict_iterate_over_conflict:
     cach_init: \<open>conflict_min_analysis_inv M' s' (NU' + NUE) D\<close> and
     NU_P_D: \<open>NU' + NUE \<Turnstile>pm add_mset K D\<close> and
     lits_D: \<open>literals_are_in_\<L>\<^sub>i\<^sub>n \<A> D\<close> and
+    lits_NU: \<open>literals_are_in_\<L>\<^sub>i\<^sub>n_mm \<A> (mset `# ran_mf NU)\<close> and
     K: \<open>K = outl ! 0\<close> and
     outl_nempty: \<open>outl \<noteq> []\<close> and
     bounded: \<open>isasat_input_bounded \<A>\<close>
@@ -2051,13 +2659,10 @@ proof -
       using \<open>E = mset (tl outl')\<close> \<open>x1d < length outl'\<close> \<open>0 < x1d\<close>
       by (auto simp: nth_in_set_tl)
 
-  have 1:
-    \<open>literal_redundant_wl_lookup \<A> M NU nxs cach ?L lbd \<le> \<Down> Id (literal_redundant_wl M NU nxs cach ?L lbd)\<close>
+    have 1:
+      \<open>literal_redundant_wl_lookup \<A> M NU nxs cach ?L lbd \<le> \<Down> (Id \<times>\<^sub>f (ana_lookups_rel NU \<times>\<^sub>f bool_rel)) (literal_redundant_wl M NU nxs cach ?L lbd)\<close>
       by (rule literal_redundant_wl_lookup_literal_redundant_wl)
-       (use n_d lits M_x1 struct_invs add_inv \<open>outl' ! x1d \<in># E\<close> \<open>E = nxs\<close> in auto)
-    then have 1:
-    \<open>literal_redundant_wl_lookup \<A> M NU nxs cach ?L lbd \<le> (literal_redundant_wl M NU nxs cach ?L lbd)\<close>
-      by simp
+       (use lits_NU n_d lits M_x1 struct_invs add_inv \<open>outl' ! x1d \<in># E\<close> \<open>E = nxs\<close> in auto)
 
     have 2:
       \<open>literal_redundant_wl M NU nxs cach ?L lbd \<le> \<Down>
@@ -2092,7 +2697,9 @@ proof -
       apply (rule order.trans)
        apply (rule 1)
       apply (rule order.trans)
+      apply (rule ref_two_step')
        apply (rule 2)
+       apply (subst conc_fun_chain)
       apply (rule order.trans)
        apply (rule ref_two_step'[OF 3])
       unfolding literal_redundant_spec_def is_literal_redundant_spec_def
@@ -2396,54 +3003,57 @@ lemma conflict_min_cach_set_removable:
       conflict_min_cach_set_removable_l_def)
 
 text \<open>This is the result of trying and discovering that MLton is able to optimise the code better.\<close>
-datatype 'n ana_ref = Ana_Ref 'n 'n 'n 'n
+datatype ('n, 'b) ana_ref = Ana_Ref 'n 'b bool
 
-instantiation ana_ref :: (default) default
+instantiation ana_ref :: (default, default) default
 begin
 
-definition default_ana_ref :: \<open>'a ana_ref\<close> where
-  \<open>default_ana_ref = Ana_Ref default default default default\<close>
+definition default_ana_ref :: \<open>('a, 'b) ana_ref\<close> where
+  \<open>default_ana_ref = Ana_Ref default default default\<close>
 
 instance
   by standard
 end
-instance ana_ref :: (heap) heap
+instance ana_ref :: (heap, heap) heap
 
 proof
   obtain to_nata where
     b: \<open>inj (to_nata :: 'a \<Rightarrow> nat)\<close>
     by blast
 
-  obtain to_natb where
-    a: \<open>inj (to_natb :: nat \<times> nat \<times> nat \<times> nat \<Rightarrow> nat)\<close>
+  obtain to_natc where
+    c: \<open>inj (to_natc :: 'b \<Rightarrow> nat)\<close>
     by blast
-  let ?f = \<open>\<lambda>x :: 'a ana_ref. case x of Ana_Ref a b c d \<Rightarrow>
-    to_natb (to_nata a, to_nata b, to_nata c, to_nata d)\<close>
+  obtain to_natb where
+    a: \<open>inj (to_natb :: nat \<times> nat \<times> bool \<Rightarrow> nat)\<close>
+    by blast
+  let ?f = \<open>\<lambda>x :: ('a, 'b) ana_ref. case x of Ana_Ref a b c \<Rightarrow>
+    to_natb (to_nata a, to_natc b, c)\<close>
   have \<open>inj ?f\<close>
     unfolding inj_on_def
     apply (intro ballI)
     apply (case_tac x, case_tac y)
-    apply (auto dest!: injD[OF a] injD[OF b])
+    apply (auto dest!: injD[OF a] injD[OF c] injD[OF b])
     done
-  then show \<open>\<exists>to_nat. inj (to_nat :: 'a ana_ref \<Rightarrow> nat)\<close>
+  then show \<open>\<exists>to_nat. inj (to_nat :: ('a, 'b) ana_ref \<Rightarrow> nat)\<close>
     by blast
 qed
 
-fun ana_ref_assn :: \<open>('a \<Rightarrow> 'b \<Rightarrow> assn) \<Rightarrow> 'a ana_ref \<Rightarrow> 'b ana_ref \<Rightarrow> assn\<close> where [simp del]:
-  \<open>ana_ref_assn r (Ana_Ref a b c d) (Ana_Ref a' b' c' d')=
-    r a a' * r b b' * r c c' * r d d'\<close>
+fun ana_ref_assn :: \<open>('a \<Rightarrow> 'b \<Rightarrow> assn) \<Rightarrow> ('a, nat) ana_ref \<Rightarrow> ('b, uint32) ana_ref \<Rightarrow> assn\<close> where [simp del]:
+  \<open>ana_ref_assn r (Ana_Ref a b c) (Ana_Ref a' b' c')=
+    r a a' * uint32_nat_assn b b' * bool_assn c c'\<close>
 
 lemma ana_ref_assn_def:
   \<open>ana_ref_assn r = (\<lambda>x y. case (x, y) of
-    (Ana_Ref a b c d, Ana_Ref a' b' c' d') \<Rightarrow>
-    r a a' * r b b' * r c c' * r d d')\<close>
+    (Ana_Ref a b c, Ana_Ref a' b' c') \<Rightarrow>
+    r a a' * uint32_nat_assn b b' * bool_assn c c')\<close>
   apply (intro ext)
   apply (case_tac  x, case_tac y)
   by (auto simp: ana_ref_assn.simps intro!: ext)
 
 definition analyse_refinement_rel where
   \<open>analyse_refinement_rel = {(x, y).
-     y = (case x of Ana_Ref a b c d \<Rightarrow> (a, b, c, d))}\<close>
+     y = (case x of Ana_Ref a b c \<Rightarrow> (a, b, c))}\<close>
 
 definition (in -)ana_refinement_assn where
   \<open>ana_refinement_assn \<equiv> hr_comp (ana_ref_assn nat_assn) analyse_refinement_rel\<close>
@@ -2455,14 +3065,14 @@ definition (in -)ana_refinement_fast_assn where
   \<open>ana_refinement_fast_assn \<equiv>
     hr_comp (ana_ref_assn uint64_nat_assn) analyse_refinement_rel\<close>
 
-lemma ex_ana_ref_split: \<open>(\<exists>\<^sub>Aba. P ba) = (\<exists>\<^sub>A a b c d. P (Ana_Ref a b c d))\<close>
+lemma ex_ana_ref_split: \<open>(\<exists>\<^sub>Aba. P ba) = (\<exists>\<^sub>A a b c. P (Ana_Ref a b c))\<close>
 proof -
-  let ?f = \<open>\<lambda>x. case x of (a, b, c, d) \<Rightarrow> P (Ana_Ref a b c d)\<close>
-  have 1: \<open>(\<exists>x. h \<Turnstile> P x) = (\<exists>a b c d. h \<Turnstile> P (Ana_Ref a b c d))\<close> for h
+  let ?f = \<open>\<lambda>x. case x of (a, b, c) \<Rightarrow> P (Ana_Ref a b c)\<close>
+  have 1: \<open>(\<exists>x. h \<Turnstile> P x) = (\<exists>a b c. h \<Turnstile> P (Ana_Ref a b c))\<close> for h
     apply auto
     apply (case_tac x)
     by auto
-  have 2: \<open>(\<exists>\<^sub>Aa b c d. P (Ana_Ref a b c d)) = (\<exists>\<^sub>Ax. ?f x)\<close>
+  have 2: \<open>(\<exists>\<^sub>Aa b c. P (Ana_Ref a b c)) = (\<exists>\<^sub>Ax. ?f x)\<close>
     unfolding ex_assn_pair_split
     by auto
   show ?thesis
@@ -2474,6 +3084,14 @@ proof -
 qed
 
 (*TODO move*)
+lemma ex_assn_def_pure_eq_start:
+  \<open>(\<exists>\<^sub>Aba. \<up> (ba = h) * P ba) = P h\<close>
+  by (subst ex_assn_def, auto)+
+
+lemma ex_assn_def_pure_eq_start':
+  \<open>(\<exists>\<^sub>Aba. \<up> (h = ba) * P ba) = P h\<close>
+  by (subst ex_assn_def, auto)+
+
 lemma ex_assn_def_pure_eq_start2:
   \<open>(\<exists>\<^sub>Aba b. \<up> (ba = h b) * P b ba) = (\<exists>\<^sub>Ab .  P b (h b))\<close>
   by (subst ex_assn_def, subst (2) ex_assn_def, auto)+
@@ -2493,23 +3111,28 @@ lemma ex_assn_def_pure_eq_start4':
 lemma ex_assn_def_pure_eq_start1:
   \<open>(\<exists>\<^sub>Aba. \<up> (ba = h b) * P ba) = (P (h b))\<close>
   by (subst ex_assn_def, auto)+
+(*End Move*)
 
 lemma ana_refinement_fast_assn_alt_def:
-  \<open>ana_refinement_fast_assn (a', b', c' , d') (Ana_Ref a b c d)  =
-  uint64_nat_assn a' a * uint64_nat_assn b' b * uint64_nat_assn c' c * uint64_nat_assn d' d\<close>
+  \<open>ana_refinement_fast_assn (a', b', c') (Ana_Ref a b c)  =
+  uint64_nat_assn a' a * uint32_nat_assn b' b * bool_assn c' c\<close>
   unfolding ana_refinement_fast_assn_def
   apply (auto simp: hr_comp_def ana_ref_assn_def analyse_refinement_rel_def
     uint64_nat_rel_def br_def pure_def ex_ana_ref_split
-    ex_assn_def_pure_eq_middle3 ex_assn_def_pure_eq_middle2
+    ex_assn_def_pure_eq_middle2 ex_assn_def_pure_eq_middle2
     ex_assn_def_pure_eq_start2 ex_assn_def_pure_eq_start1
+    ex_assn_def_pure_eq_middle3 uint32_nat_rel_def br_def
     simp flip: merge_pure_star
     cong: )
   apply (subst star_assoc)+
-  apply (subst ex_assn_def_pure_eq_start1)
+  apply (subst ex_assn_def_pure_eq_start3)
+  apply (subst ex_assn_def_pure_eq_start2)
+  apply (subst ex_assn_def_pure_eq_start')
   by auto
+
 lemma ana_refinement_fast_assn_alt_def2:
-  \<open>ana_refinement_fast_assn = (\<lambda>(a', b', c' , d') x. case x of (Ana_Ref a b c d) \<Rightarrow>
-  uint64_nat_assn a' a * uint64_nat_assn b' b * uint64_nat_assn c' c * uint64_nat_assn d' d)\<close>
+  \<open>ana_refinement_fast_assn = (\<lambda>(a', b', c') x. case x of (Ana_Ref a b c) \<Rightarrow>
+  uint64_nat_assn a' a * uint32_nat_assn b' b * bool_assn c' c)\<close>
   apply (auto simp: ana_refinement_fast_assn_alt_def intro!: ext)
   apply (case_tac x)
   by (auto simp: ana_refinement_fast_assn_alt_def intro!: ext)
@@ -2518,8 +3141,8 @@ lemma ex_assn_cong:
   by auto
 
 lemma ana_refinement_assn_alt_def:
-  \<open>ana_refinement_assn (a', b', c' , d') (Ana_Ref a b c d)  =
-  nat_assn a' a * nat_assn b' b * nat_assn c' c * nat_assn d' d\<close>
+  \<open>ana_refinement_assn (a', b', c') (Ana_Ref a b c)  =
+  nat_assn a' a * uint32_nat_assn b' b * bool_assn c' c\<close>
   unfolding ana_refinement_assn_def
   apply (auto simp: hr_comp_def ana_ref_assn_def analyse_refinement_rel_def
     uint64_nat_rel_def br_def pure_def ex_ana_ref_split
@@ -2527,16 +3150,17 @@ lemma ana_refinement_assn_alt_def:
     ex_assn_def_pure_eq_start2 ex_assn_def_pure_eq_start1
       ex_assn_def_pure_eq_start3
       ex_assn_def_pure_eq_start3'
-      ex_assn_def_pure_eq_start4'
+      ex_assn_def_pure_eq_start4' uint32_nat_rel_def br_def
       eq_commute[of a] eq_commute[of b] eq_commute[of c] eq_commute[of d]
     simp flip: merge_pure_star
     cong: ex_assn_cong)
   apply (subst star_assoc)+
-  apply (subst ex_assn_def_pure_eq_start1)
+  apply (subst ex_assn_def_pure_eq_start)
   by auto
+
 lemma ana_refinement_assn_alt_def2:
-  \<open>ana_refinement_assn = (\<lambda>(a', b', c' , d') x. case x of (Ana_Ref a b c d) \<Rightarrow>
-  nat_assn a' a * nat_assn b' b * nat_assn c' c * nat_assn d' d)\<close>
+  \<open>ana_refinement_assn = (\<lambda>(a', b', c') x. case x of (Ana_Ref a b c) \<Rightarrow>
+  nat_assn a' a * uint32_nat_assn b' b * bool_assn c' c)\<close>
   apply (auto simp: ana_refinement_assn_alt_def intro!: ext)
   apply (case_tac x)
   by (auto simp: ana_refinement_assn_alt_def intro!: ext)
@@ -2544,8 +3168,9 @@ lemma ana_refinement_assn_alt_def2:
 lemma [safe_constraint_rules]: \<open>CONSTRAINT is_pure ana_refinement_assn\<close>
   unfolding CONSTRAINT_def is_pure_def
   supply[[show_sorts]]
-  apply (rule exI[of _ \<open>\<lambda>x x'. (x :: nat \<times> nat \<times> nat \<times> nat) = (case x' of
-    Ana_Ref a b c d \<Rightarrow> (a, b, c , d))\<close>])
+  apply (rule exI[of _ \<open>\<lambda>(a, b, c) x'. (case x' of
+    Ana_Ref a' b' c' \<Rightarrow> (a', a) \<in> nat_rel \<and> (b', b) \<in> uint32_nat_rel \<and>
+      (c', c) \<in> bool_rel)\<close>])
   apply (auto simp: is_pure_def ana_refinement_assn_alt_def2)
   apply (case_tac x')
   by (auto simp: pure_def)
@@ -2553,9 +3178,9 @@ lemma [safe_constraint_rules]: \<open>CONSTRAINT is_pure ana_refinement_assn\<cl
 lemma [safe_constraint_rules]: \<open>CONSTRAINT is_pure ana_refinement_fast_assn\<close>
   unfolding CONSTRAINT_def is_pure_def
   supply[[show_sorts]]
-  apply (rule exI[of _ \<open>\<lambda>(a, b, c , d) x'.  (case x' of
-    Ana_Ref a' b' c' d' \<Rightarrow> (a', a) \<in> uint64_nat_rel \<and> (b', b) \<in> uint64_nat_rel \<and>
-      (c', c) \<in> uint64_nat_rel \<and> (d', d) \<in> uint64_nat_rel)\<close>])
+  apply (rule exI[of _ \<open>\<lambda>(a, b, c) x'.  (case x' of
+    Ana_Ref a' b' c' \<Rightarrow> (a', a) \<in> uint64_nat_rel \<and> (b', b) \<in> uint32_nat_rel \<and>
+      (c', c) \<in> bool_rel)\<close>])
   apply (auto simp: is_pure_def ana_refinement_fast_assn_alt_def2)
   apply (case_tac x')
   by (auto simp: pure_def)
@@ -2565,20 +3190,20 @@ abbreviation (in -)analyse_refinement_fast_assn where
     arl_assn ana_refinement_fast_assn\<close>
 
 definition to_ana_ref_id where
-  [simp]: \<open>to_ana_ref_id = (\<lambda>a b c d. (a, b, c, d))\<close>
+  [simp]: \<open>to_ana_ref_id = (\<lambda>a b c. (a, b, c))\<close>
 
 definition to_ana_ref where
-  \<open>to_ana_ref = (\<lambda>a b c d. Ana_Ref a b c d)\<close>
+  \<open>to_ana_ref = (\<lambda>a b c. Ana_Ref a b c)\<close>
 
 definition from_ana_ref_id where
   [simp]: \<open>from_ana_ref_id x = x\<close>
 
 definition from_ana_ref where
-  \<open>from_ana_ref = (\<lambda>x. case x of Ana_Ref a b c d \<Rightarrow> (a, b, c, d))\<close>
+  \<open>from_ana_ref = (\<lambda>x. case x of Ana_Ref a b c \<Rightarrow> (a, b, c))\<close>
 
 lemma to_ana_ref_id_fast_hnr[sepref_fr_rules]:
-  \<open>(uncurry3 (return oooo to_ana_ref), uncurry3 (RETURN oooo to_ana_ref_id)) \<in>
-   uint64_nat_assn\<^sup>k *\<^sub>a uint64_nat_assn\<^sup>k *\<^sub>a uint64_nat_assn\<^sup>k *\<^sub>a uint64_nat_assn\<^sup>k \<rightarrow>\<^sub>a
+  \<open>(uncurry2 (return ooo to_ana_ref), uncurry2 (RETURN ooo to_ana_ref_id)) \<in>
+   uint64_nat_assn\<^sup>k *\<^sub>a uint32_nat_assn\<^sup>k *\<^sub>a bool_assn\<^sup>k \<rightarrow>\<^sub>a
    ana_refinement_fast_assn\<close>
  by sepref_to_hoare
    (sep_auto simp: to_ana_ref_def to_ana_ref_id_def ana_ref_assn_def
@@ -2586,19 +3211,19 @@ lemma to_ana_ref_id_fast_hnr[sepref_fr_rules]:
    case_prod_beta ana_refinement_fast_assn_alt_def pure_def)
 
 lemma to_ana_ref_id_hnr[sepref_fr_rules]:
-  \<open>(uncurry3 (return oooo to_ana_ref), uncurry3 (RETURN oooo to_ana_ref_id)) \<in>
-   nat_assn\<^sup>k *\<^sub>a nat_assn\<^sup>k *\<^sub>a nat_assn\<^sup>k *\<^sub>a nat_assn\<^sup>k \<rightarrow>\<^sub>a
+  \<open>(uncurry2 (return ooo to_ana_ref), uncurry2 (RETURN ooo to_ana_ref_id)) \<in>
+   nat_assn\<^sup>k *\<^sub>a uint32_nat_assn\<^sup>k *\<^sub>a bool_assn\<^sup>k \<rightarrow>\<^sub>a
    ana_refinement_assn\<close>
   unfolding ana_refinement_assn_alt_def[abs_def]
  by sepref_to_hoare
    (sep_auto simp: to_ana_ref_def to_ana_ref_id_def
     uint64_nat_rel_def br_def ana_refinement_assn_alt_def
-   case_prod_beta  pure_def)
+   case_prod_beta pure_def)
 
 lemma [sepref_fr_rules]:
   \<open>((return o from_ana_ref), (RETURN o from_ana_ref_id)) \<in>
    ana_refinement_fast_assn\<^sup>k \<rightarrow>\<^sub>a
-   uint64_nat_assn *a uint64_nat_assn *a uint64_nat_assn *a uint64_nat_assn\<close>
+   uint64_nat_assn *a uint32_nat_assn *a bool_assn\<close>
   apply sepref_to_hoare
   apply (case_tac xi)
   apply
@@ -2610,7 +3235,7 @@ lemma [sepref_fr_rules]:
 lemma [sepref_fr_rules]:
   \<open>((return o from_ana_ref), (RETURN o from_ana_ref_id)) \<in>
    ana_refinement_assn\<^sup>k \<rightarrow>\<^sub>a
-  nat_assn *a nat_assn *a nat_assn *a nat_assn\<close>
+  nat_assn *a uint32_nat_assn *a bool_assn\<close>
   unfolding ana_refinement_assn_alt_def[abs_def]
   apply sepref_to_hoare
   apply (case_tac xi)
@@ -2633,7 +3258,7 @@ definition isa_mark_failed_lits_stack where
       (\<lambda>(i, cach). i < l)
       (\<lambda>(i, cach). do {
         ASSERT(i < length analyse);
-        let (cls_idx, _, idx, _) = from_ana_ref_id (analyse ! i);
+        let (cls_idx, idx, _) = from_ana_ref_id (analyse ! i);
         ASSERT(cls_idx + idx \<ge> 1);
         ASSERT(cls_idx + idx - 1 < length NU);
 	ASSERT(arena_lit_pre NU (cls_idx + idx - 1));
@@ -2664,7 +3289,7 @@ private lemma mark_failed_lits_stack_inv_helper2: \<open>mark_failed_lits_stack_
 lemma isa_mark_failed_lits_stack_isa_mark_failed_lits_stack:
   \<open>(uncurry2 isa_mark_failed_lits_stack, uncurry2 (mark_failed_lits_stack \<A>\<^sub>i\<^sub>n)) \<in>
      [\<lambda>((N, ana), cach). True]\<^sub>f
-     {(arena, N). valid_arena arena N vdom} \<times>\<^sub>f Id \<times>\<^sub>f cach_refinement \<A>\<^sub>i\<^sub>n \<rightarrow>
+     {(arena, N). valid_arena arena N vdom} \<times>\<^sub>f ana_lookups_rel NU \<times>\<^sub>f cach_refinement \<A>\<^sub>i\<^sub>n \<rightarrow>
      \<langle>cach_refinement \<A>\<^sub>i\<^sub>n\<rangle>nres_rel\<close>
 proof -
   have [refine0]: \<open>((0, x2c), 0, x2a) \<in> nat_rel \<times>\<^sub>f cach_refinement \<A>\<^sub>i\<^sub>n\<close>
@@ -2685,7 +3310,8 @@ proof -
       ge1: \<open>x1g + x2g \<ge> 1\<close>
     if
       \<open>case y of (x, xa) \<Rightarrow> (case x of (N, ana) \<Rightarrow> \<lambda>cach. True) xa\<close> and
-      xy: \<open>(x, y) \<in> {(arena, N). valid_arena arena N vdom} \<times>\<^sub>f Id \<times>\<^sub>f cach_refinement \<A>\<^sub>i\<^sub>n\<close> and
+      xy: \<open>(x, y) \<in> {(arena, N). valid_arena arena N vdom} \<times>\<^sub>f ana_lookups_rel NU
+         \<times>\<^sub>f cach_refinement \<A>\<^sub>i\<^sub>n\<close> and
       st:
         \<open>x1 = (x1a, x2)\<close>
         \<open>y = (x1, x2a)\<close>
@@ -2696,15 +3322,13 @@ proof -
 	\<open>x2f2 = (x2f, x2f3)\<close>
 	\<open>x2f0 = (x2f1, x2f2)\<close>
         \<open>x2 ! x1d = (x1f, x2f0)\<close>
-	\<open>x2g2 = (x2g, x2g3)\<close>
-	\<open>x2g0 = (x2g1, x2g2)\<close>
+	\<open>x2g0 = (x2g, x2g2)\<close>
         \<open>x2b ! x1e = (x1g, x2g0)\<close> and
       xax': \<open>(xa, x') \<in> nat_rel \<times>\<^sub>f cach_refinement \<A>\<^sub>i\<^sub>n\<close> and
       cond: \<open>case xa of (i, cach) \<Rightarrow> i < length x2b\<close> and
       cond': \<open>case x' of (i, cach) \<Rightarrow> i < length x2\<close> and
       inv: \<open>case x' of (_, x) \<Rightarrow> mark_failed_lits_stack_inv x1a x2 x\<close> and
-      \<open>x1d < length x2\<close> and
-      le: \<open>x1e < length x2b\<close> and
+      le: \<open>x1d < length x2\<close> \<open>x1e < length x2b\<close> and
       atm: \<open>atm_of (x1a \<propto> x1f ! (x2f - 1)) \<in># \<A>\<^sub>i\<^sub>n\<close>
     for x y x1 x1a x2 x2a x1b x1c x2b x2c xa x' x1d x2d x1e x2e x1f x2f x1g x2g
       x2f0 x2f1 x2f2 x2f3 x2g0 x2g1 x2g2 x2g3
@@ -2713,24 +3337,22 @@ proof -
     have [simp]:
       \<open>x1 = (x1a, x2)\<close>
       \<open>y = ((x1a, x2), x2a)\<close>
-      \<open>x1b = (x1c, x2)\<close>
-      \<open>x = ((x1c, x2), x2c)\<close>
+      \<open>x1b = (x1c, x2b)\<close>
+      \<open>x = ((x1c, x2b), x2c)\<close>
       \<open>x' = (x1d, x2d)\<close>
       \<open>xa = (x1d, x2e)\<close>
       \<open>x1f = x1g\<close>
-      \<open>x2f = x2g\<close>
-      \<open>x2f1 = x2g1\<close>
-      \<open>x2f0 = x2g0\<close>
       \<open>x1e = x1d\<close>
-      \<open>x2g0 = (x2g1, x2g, x2g3)\<close>
-      \<open>x2f3 = x2g3\<close>
-      \<open>x2f2 = x2g2\<close>
-      \<open>x2b = x2\<close> and
-      st': \<open>x2 ! x1d = (x1g, x2g0)\<close> and
+      \<open>x2f0 = (x2f1, x2f, x2f3)\<close>
+      \<open>x2g = x2f\<close>
+      \<open>x2g0 = (x2g, x2g2)\<close> and
+      st': \<open>x2 ! x1d = (x1g, x2f0)\<close> and
       cach:\<open>(x2e, x2d) \<in> cach_refinement \<A>\<^sub>i\<^sub>n\<close> and
-      \<open>(x2c, x2a) \<in> cach_refinement \<A>\<^sub>i\<^sub>n\<close>
-      using xy st xax'
-      by auto
+      \<open>(x2c, x2a) \<in> cach_refinement \<A>\<^sub>i\<^sub>n\<close> and
+      x2f0_x2g0: \<open>((x1g, x2g, x2g2), (x1f, x2f1, x2f, x2f3)) \<in> ana_lookup_rel NU\<close>
+      using xy st xax' param_nth[of x1e x2 x1d x2b \<open>ana_lookup_rel NU\<close>] le
+      by (auto intro: simp: ana_lookup_rel_alt_def)
+
     have arena: \<open>valid_arena x1c x1a vdom\<close>
       using xy unfolding st by auto
     have \<open>x2 ! x1e \<in> set x2\<close>
@@ -2739,26 +3361,31 @@ proof -
     then have \<open>x2 ! x1d \<in> set x2\<close> and
       x2f: \<open>x2f \<le> length (x1a \<propto> x1f)\<close> and
       x1f: \<open>x1g \<in># dom_m x1a\<close> and
-      x2g: \<open>x2g > 0\<close>
-      using inv le unfolding mark_failed_lits_stack_inv_def x' prod.case st st'
-      by (auto simp del: nth_mem simp: st')
+      x2g: \<open>x2g > 0\<close> and
+      x2g_u1_le: \<open>x2g - 1 < length (x1a \<propto> x1f)\<close>
+      using inv le x2f0_x2g0 nth_mem[of x1d x2]
+      unfolding mark_failed_lits_stack_inv_def x' prod.case st st'
+      by (auto simp del: nth_mem simp: st' ana_lookup_rel_alt_def split: if_splits
+        dest!: bspec[of \<open>set x2\<close> _ \<open>(_, _, _, _)\<close>])
+
     have \<open>is_Lit (x1c ! (x1g + (x2g - 1)))\<close>
-      by (rule arena_lifting[OF arena x1f]) (use x2f x2g in auto)
+      by (rule arena_lifting[OF arena x1f]) (use x2f x2g x2g_u1_le in auto)
     then show ?le and ?A
-      using arena_lifting[OF arena x1f] le x2f x1f x2g atm by (auto simp: arena_lit_def)
+      using arena_lifting[OF arena x1f] le x2f x1f x2g atm x2g_u1_le
+      by (auto simp: arena_lit_def)
     show ?lit
       unfolding arena_lit_pre_def arena_is_valid_clause_idx_and_access_def
       by (rule bex_leI[of _ x1f])
-        (use arena x1f x2f x2g in \<open>auto intro!: exI[of _ x1a] exI[of _ vdom]\<close>)
+        (use arena x1f x2f x2g x2g_u1_le in \<open>auto intro!: exI[of _ x1a] exI[of _ vdom]\<close>)
     show \<open>x1g + x2g \<ge> 1\<close>
       using x2g by auto
     have [simp]: \<open>arena_lit x1c (x1g + x2g - Suc 0) = x1a \<propto> x1g ! (x2g - Suc 0)\<close>
-       using that x1f x2f x2g by (auto simp: arena_lifting[OF arena])
+       using that x1f x2f x2g x2g_u1_le by (auto simp: arena_lifting[OF arena])
     have \<open>atm_of (arena_lit x1c (x1g + x2g - Suc 0)) < length (fst x2e)\<close>
       using \<open>?A\<close> cach by (auto simp: cach_refinement_alt_def dest: multi_member_split)
 
     then show ?final
-      using \<open>?le\<close> \<open>?A\<close> cach
+      using \<open>?le\<close> \<open>?A\<close> cach x1f x2g_u1_le x2g
       by (cases x2e)
         (auto simp: conflict_min_cach_set_failed_l_def cach_refinement_alt_def
         arena_lifting[OF arena])
@@ -2772,7 +3399,8 @@ proof -
     apply refine_vcg
     subgoal by auto
     subgoal by auto
-    subgoal by auto
+    subgoal for x y x1 x1a x2 x2a x1b x1c x2b x2c xa x' x1d x2d x1e x2e
+      by (auto simp: list_rel_imp_same_length)
     subgoal by auto
     subgoal by (rule ge1)
     subgoal by (rule le_length_arena)
@@ -2799,6 +3427,7 @@ sepref_definition isa_mark_failed_lits_stack_code
     nth_rll_def[symmetric]
     fmap_rll_def[symmetric]
     conflict_min_cach_set_failed_l_def
+  apply (rewrite at \<open>arena_lit _ (_ + \<hole> - _)\<close> nat_of_uint32_conv_def[symmetric])
   by sepref
 
 
@@ -2819,6 +3448,7 @@ sepref_definition isa_mark_failed_lits_stack_fast_code
     fmap_rll_def[symmetric]
     arena_lit_def[symmetric]
     conflict_min_cach_set_failed_l_def
+  apply (rewrite at \<open>arena_lit _ (_ + \<hole> - _)\<close> uint64_of_uint32_conv_def[symmetric])
   apply (rewrite in \<open>_ - \<hole>\<close> one_uint64_nat_def[symmetric])
   apply (rewrite in \<open>_ - \<hole>\<close> one_uint64_nat_def[symmetric])
   apply (rewrite in \<open>_ - \<hole>\<close> one_uint64_nat_def[symmetric])
@@ -2831,16 +3461,16 @@ declare isa_mark_failed_lits_stack_code.refine[sepref_fr_rules]
 declare isa_mark_failed_lits_stack_fast_code.refine[sepref_fr_rules]
 
 definition isa_get_literal_and_remove_of_analyse_wl
-   :: \<open>arena \<Rightarrow> (nat \<times> nat \<times> nat \<times> nat) list \<Rightarrow> nat literal \<times> (nat \<times> nat \<times> nat \<times> nat) list\<close> where
+   :: \<open>arena \<Rightarrow> (nat \<times> nat \<times> bool) list \<Rightarrow> nat literal \<times> (nat \<times> nat \<times> bool) list\<close> where
   \<open>isa_get_literal_and_remove_of_analyse_wl C analyse =
-    (let (i, k, j, len) = from_ana_ref_id (last analyse) in
-     (arena_lit C (i + j), analyse[length analyse - 1 := to_ana_ref_id i k (j + 1) len]))\<close>
+    (let (i, j, b) = from_ana_ref_id (last analyse) in
+     (arena_lit C (i + j), analyse[length analyse - 1 := to_ana_ref_id i (j + 1) b]))\<close>
 
 definition isa_get_literal_and_remove_of_analyse_wl_pre
-   :: \<open>arena \<Rightarrow> (nat \<times> nat \<times> nat \<times> nat) list \<Rightarrow> bool\<close> where
+   :: \<open>arena \<Rightarrow> (nat \<times> nat \<times> bool) list \<Rightarrow> bool\<close> where
 \<open>isa_get_literal_and_remove_of_analyse_wl_pre arena analyse \<longleftrightarrow>
-  (let (i, k, j, len) = last analyse in
-    analyse \<noteq> [] \<and> arena_lit_pre arena (i+j))\<close>
+  (let (i, j, b) = last analyse in
+    analyse \<noteq> [] \<and> arena_lit_pre arena (i+j) \<and> i + j < uint32_max)\<close>
 
 sepref_register to_ana_ref_id
 sepref_definition isa_get_literal_and_remove_of_analyse_wl_code
@@ -2849,7 +3479,9 @@ sepref_definition isa_get_literal_and_remove_of_analyse_wl_code
       arena_assn\<^sup>k *\<^sub>a analyse_refinement_assn\<^sup>d \<rightarrow>
       unat_lit_assn *a analyse_refinement_assn\<close>
   unfolding isa_get_literal_and_remove_of_analyse_wl_pre_def
-  isa_get_literal_and_remove_of_analyse_wl_def fast_minus_def[symmetric]
+    isa_get_literal_and_remove_of_analyse_wl_def fast_minus_def[symmetric]
+  apply (rewrite at \<open>arena_lit _ (_ + \<hole>)\<close> nat_of_uint32_conv_def[symmetric])
+  apply (rewrite at \<open>(_ + \<hole>)\<close> one_uint32_nat_def[symmetric])
   by sepref
 
 lemma arena_lit_pre_le: \<open>length a \<le> uint64_max \<Longrightarrow>
@@ -2871,7 +3503,8 @@ sepref_definition isa_get_literal_and_remove_of_analyse_wl_fast_code
   supply [[goals_limit=1]] arena_lit_pre_le2[dest]
   unfolding isa_get_literal_and_remove_of_analyse_wl_pre_def
   isa_get_literal_and_remove_of_analyse_wl_def fast_minus_def[symmetric]
-  apply (rewrite at \<open>_ + \<hole>\<close> one_uint64_nat_def[symmetric])
+  apply (rewrite at \<open>_ + \<hole>\<close> one_uint32_nat_def[symmetric])
+  apply (rewrite at \<open>arena_lit _ (_ + \<hole>)\<close> uint64_of_uint32_conv_def[symmetric])
   by sepref
 
 declare isa_get_literal_and_remove_of_analyse_wl_code.refine[sepref_fr_rules]
@@ -2883,13 +3516,13 @@ definition lit_redundant_reason_stack_wl_lookup_pre :: \<open>nat literal \<Righ
   arena_is_valid_clause_idx NU C\<close>
 
 definition lit_redundant_reason_stack_wl_lookup
-  :: \<open>nat literal \<Rightarrow> arena_el list \<Rightarrow> nat \<Rightarrow> nat \<times> nat \<times> nat \<times> nat\<close>
+  :: \<open>nat literal \<Rightarrow> arena_el list \<Rightarrow> nat \<Rightarrow> nat \<times> nat \<times> bool\<close>
 where
 \<open>lit_redundant_reason_stack_wl_lookup L NU C =
-  (if arena_length NU C > 2 then to_ana_ref_id C 0 1 (arena_length NU C)
+  (if arena_length NU C > 2 then to_ana_ref_id C 1 False
   else if arena_lit NU C = L
-  then to_ana_ref_id C 0 1 (arena_length NU C)
-  else to_ana_ref_id C 1 0 1)\<close>
+  then to_ana_ref_id C 1 False
+  else to_ana_ref_id C 0 True)\<close>
 
 definition isa_lit_redundant_rec_wl_lookup
   :: \<open>trail_pol \<Rightarrow> arena \<Rightarrow> lookup_clause_rel \<Rightarrow>
@@ -2900,7 +3533,7 @@ where
         (\<lambda>(cach, analyse, b). analyse \<noteq> [])
         (\<lambda>(cach, analyse, b). do {
             ASSERT(analyse \<noteq> []);
-	    let (C, k, i, len) = from_ana_ref_id (last analyse);
+	    let (C, i, len) = from_ana_ref_id (last analyse);
             ASSERT(C < length NU);
             ASSERT(arena_is_valid_clause_idx NU C);
             ASSERT(arena_lit_pre NU (C + k));
@@ -3784,14 +4417,6 @@ definition isasat_lookup_merge_eq2
     RETURN((False, zs), clvls, lbd, outl)
   })\<close>
 
-(*TODO Move*)
-lemma literals_are_in_\<L>\<^sub>i\<^sub>n_mm_add_msetD:
-  \<open>literals_are_in_\<L>\<^sub>i\<^sub>n_mm \<A> (add_mset C N) \<Longrightarrow>
-  L \<in># C \<Longrightarrow> L \<in># \<L>\<^sub>a\<^sub>l\<^sub>l \<A>\<close>
-  by (auto simp: literals_are_in_\<L>\<^sub>i\<^sub>n_mm_def all_lits_of_mm_add_mset
-      all_lits_of_m_add_mset
-    dest!: multi_member_split)
-
 lemma isasat_lookup_merge_eq2_lookup_merge_eq2:
   assumes valid: \<open>valid_arena arena N vdom\<close> and i: \<open>i \<in># dom_m N\<close> and
     lits: \<open>literals_are_in_\<L>\<^sub>i\<^sub>n_mm \<A> (mset `# ran_mf N)\<close> and
@@ -3910,13 +4535,6 @@ definition merge_conflict_m_eq2_pre where
 
 definition merge_conflict_m_g_eq2 :: \<open>_\<close> where
 \<open>merge_conflict_m_g_eq2 L M N i D _ _ _ = merge_conflict_m_eq2 L M (N \<propto> i) D\<close>
-
-lemma literals_are_in_\<L>\<^sub>i\<^sub>n_mm_add_mset:
-  \<open>literals_are_in_\<L>\<^sub>i\<^sub>n_mm \<A> (add_mset C N) \<longleftrightarrow>
-    literals_are_in_\<L>\<^sub>i\<^sub>n_mm \<A> N \<and> literals_are_in_\<L>\<^sub>i\<^sub>n \<A> C\<close>
-  unfolding literals_are_in_\<L>\<^sub>i\<^sub>n_mm_def
-    literals_are_in_\<L>\<^sub>i\<^sub>n_def
-  by (auto simp: all_lits_of_mm_add_mset)
 
 lemma isasat_lookup_merge_eq2:
   \<open>(uncurry7 isasat_lookup_merge_eq2, uncurry7 merge_conflict_m_g_eq2) \<in>
